Cleaning up the complexity file

src/complexity/basic.lean
@@ -1,255 +1,45 @@
-import tactic.basic
-import computability.encoding
-import computability.tm_computable
-
--- Useful lemmas for dealing with function types
-lemma ftype {α α': Type} {β β': Type}: α = α' → β = β' → (α → β) = (α' → β') :=
-by { intros p q, rw [p, q] }
-
-lemma ftype_right (α: Type) {β β': Type}: β = β' → (α → β) = (α → β') :=
-by { intro p, rw [p] }
-
-lemma fcast: ∀ {α β γ: Type} (f: α → β) (a: α) (h: (β = γ)), (cast h (f a)) = (cast (ftype_right α h) f) a :=
- by { intros α β γ f a h, finish }
-
- lemma fcast': ∀ {α β γ: Type} (f: α → β) (a: α) (h: (β = γ)) (h': ((α → β) = (α → γ))), (cast h (f a)) = (cast h' f) a :=
- by { intros α β γ f a h, finish }
+import tactic
 
 namespace complexity
 
-/- Complexity is defined in terms of a model of program and data.
- - The model is provided a function that checks the cost of the computing a given output
- -  another function that applies some data as an argument to the program
- - The accepts_with_cost function can only return a single result
- -
- - Data can be converted from lean types into the data type using the
- -  has_encoding class
- -/
+structure model :=
+  (Program Data Result Cost: Type*)
+  (data_equiv: setoid Data)
+  (result_equiv: setoid Result)
+  (cost_lt: preorder Cost)
+  (cost_add: has_add Cost)
+  (apply: Program → Data → Program)
+  (has_cost: Program → Cost → Prop)
+  (result: Π {p c}, (has_cost p c) → Result)
+  (cost_pos: ∀ (c₀ c₁: Cost), c₀ ≤ c₀ + c₁)
+  (has_cost_mono: ∀ p c₀ c₁, has_cost p c₀ → c₀ ≤ c₁ → has_cost p c₁)
 
-structure model (α β γ: Type*) [has_equiv β]  [preorder γ]  [has_add γ] :=
-mk ::
-  (accepts_with_cost : α → β → γ → Prop)
-  (application : α → β → α)
-  (cost_inj: ∀ {a: α} {b₀ b₁: β} {c₀ c₁: γ}, accepts_with_cost a b₀ c₀ → accepts_with_cost a b₁ c₁ → b₀ ≈ b₁)
-  (cost_mono : ∀ {a : α} {b : β} {c₀ c₁ : γ}, c₀ ≤ c₁ → accepts_with_cost a b c₀ → accepts_with_cost a b c₁)
+instance (m: model): setoid m.Data := m.data_equiv
+instance (m: model): setoid m.Result := m.result_equiv
+instance (m: model): preorder m.Cost := m.cost_lt
+instance (m: model): has_add m.Cost := m.cost_add
 
-universes u₀ u₁ u₂
-variables {α: Type u₀} {β: Type u₁} {γ: Type u₂} [has_equiv β] [preorder γ] [has_add γ]
+class has_encoding (α: Type*) (Data: Type*) [setoid Data] :=
+  (encode: α → Data)
+  (inj: ∀ {a b}, ⟦encode a⟧ = ⟦encode b⟧ → a = b)
 
-namespace model
-@[simp] def program_type: model α β γ → Type u₀ := λ _, α
-@[simp] def data_type: model α β γ → Type u₁ := λ _, β
-@[simp] def cost_type: model α β γ → Type u₂ := λ _, γ
-end model
+def encode {α: Type*} {Data: Type*} [setoid Data] [has_encoding α Data]: α → Data := has_encoding.encode
 
-structure encoding (m: model α β γ) (δ: Type*) :=
-mk ::
-  (encode: δ → β)
-  (encode_inj: ∀ x y: δ, encode x ≈ encode y ↔ x = y)
+theorem encode_inj {α: Type*} {Data: Type*} [setoid Data] [has_encoding α Data]
+  {a b: α}: ⟦(encode a:Data)⟧ = ⟦encode b⟧ → a = b := has_encoding.inj
 
-variables {m: model α β γ}
+theorem encode_inj_iff {α: Type*} {Data: Type*} [setoid Data] [has_encoding α Data]
+  {a b: α}: ⟦(encode a:Data)⟧ = ⟦encode b⟧ ↔ a = b := ⟨ encode_inj, λ h, h ▸ rfl ⟩
 
-namespace encoding
-variables {δ: Type*}
-
-@[simp] def model : encoding m δ → model α β γ := λ _,  m
-@[simp] def type : encoding m δ → Type* := λ _, δ
-
-@[simp] def application (en: encoding m δ) (prog: α) (arg: δ): α :=
-  en.model.application prog (en.encode arg)
-
-@[simp] theorem inj_iff (en: encoding m δ) (a b: δ):
-  en.encode a ≈ en.encode b ↔ a = b := en.encode_inj _ _
-end encoding
-
-class has_encoding (m: model α β γ) (δ: Type*) := (value: encoding m δ)
-
-def encode (m: model α β γ) {δ: Type} [f: has_encoding m δ] := f.value.encode
-
-inductive encodable_function (m: model α β γ)
-| result: Π {δ: Type}, encoding m δ → encodable_function
-| application: Π {δ: Type}, encoding m δ → encodable_function → encodable_function
-
-namespace encodable_function
-@[simp] def model : encodable_function m → model α β γ := λ _, m
-
-@[simp] def unwrap: encodable_function m → Type
-| (result en) := en.type
-| (application en b) := en.type → b.unwrap
-
-@[simp] def result_type: encodable_function m → Type
-| (result en) := en.type
-| (application _ b) := b.result_type
-
-def with_result (δ: Type*): encodable_function m → Type*
-| (result _) := δ
-| (@application _ _ _ _ _ _ _ t _ f) := t → with_result f
-
-end encodable_function
-variables {enf: encodable_function m}
-
-
-structure is_encoded_function (m: model α β γ) (δ: Type):=
-mk ::
-  (value: encodable_function m)
-  (sound: value.unwrap = δ)
-
-class has_encodable_function (m: model α β γ) (δ: Type) := (value: is_encoded_function m δ)
-
-variables {δ: Type} [has_encodable_function m δ]
-
-@[simp] theorem unwrap_has_encodable (a: has_encodable_function m δ): a.value.value.unwrap = δ := a.value.sound
-theorem unwrap_has_encodable' (a: has_encodable_function m δ): δ = a.value.value.unwrap := a.value.sound.symm
-
-@[simp] theorem unwrap_is_encoded_function (a: is_encoded_function m δ): a.value.unwrap = δ := a.sound
-
-def cast_unwrap [a: has_encodable_function m δ] (f: δ): a.value.value.unwrap :=
-  cast (unwrap_has_encodable' a) f
-
-instance encodable_result (δ: Type) [f: has_encoding m δ]:
-    has_encodable_function m δ :=
-  ⟨ ⟨ encodable_function.result f.value, rfl ⟩ ⟩
-
-instance encodable_application (δ: Type) [f: has_encoding m δ] (ε: Type) [g: has_encodable_function m ε]:
-    has_encodable_function m (δ → ε) :=
-  ⟨ ⟨ encodable_function.application f.value g.value.value, ftype rfl g.value.sound ⟩ ⟩
-
-def result_type (m: model α β γ) (δ: Type) [f: has_encodable_function m δ] := f.value.value.result_type
-
-def with_result' (m: model α β γ) (δ :Type) (η: Type*) [ef: has_encodable_function m δ]: Type* :=
-  encodable_function.with_result δ ef.value.value
-
-def cost_function: encodable_function m → Type u₂
-| (encodable_function.result _) := γ
-| (encodable_function.application en c) := en.type → cost_function c
-
-@[simp] def cost_function' (m: model α β γ) (δ : Type) [f: has_encodable_function m δ] := cost_function f.value.value
-
-namespace cost_function
-variables {cf₀ cf₁ : cost_function enf}
-
-def less_than_or_equal: Π {enf: encodable_function m}, cost_function enf → cost_function enf → Prop
-| (encodable_function.result _) := λ n m: γ, n ≤ m
-| (encodable_function.application _ _) := λ f g, ∀ a, less_than_or_equal (f a) (g a)
-
-instance: preorder (cost_function enf) := begin
-  fconstructor,
-  exact cost_function.less_than_or_equal,
-  induction enf,
-  { intro cf, refl },
-  { intros cf x, exact enf_ih _ },
-  induction enf,
-  { intros a b c,
-    apply preorder.le_trans},
-  { intros a b c hab hac x,
-    exact enf_ih _ _ _ (hab x) (hac x) },
-end
-
-def add: Π {enf: encodable_function m}, cost_function enf → cost_function enf → cost_function enf
-| (encodable_function.result _) := λ n m: γ, (n + m: γ)
-| (encodable_function.application _ _) := λ f g a, add (f a) (g a)
-
-instance add_costs: has_add (cost_function enf) := ⟨ add ⟩
-
-def lift: Π (enf: encodable_function m), γ → cost_function enf
-| (encodable_function.result _) := λ c, c
-| (encodable_function.application _ enf) := λ c _, lift enf c
-
-instance lift_costs: has_lift γ (cost_function enf) := ⟨ lift enf ⟩
-
--- theorem add_lift 
---   {φ: Type} [en: has_encoding m φ]
---   {ψ: Type} [enf: has_encodable_function m (φ → ψ)]
---   (cf: cost_function enf.) (c: γ):
--- begin
---  apply @eq (cost_function (encodable_function.application en.value enf)),
---  apply has_add.add _ _,
---  apply_instance,
---  exact (λ b, cf),
---  apply cost_function.lift begin
---   apply has_encodable_function.value.value,
---   swap,
-  
---  end,
---  apply c,
---  refine (λ b, _),
---  apply has_add.add _ _,
---  apply_instance,
---  apply cf,
---  apply cost_function.lift,
---  apply c,
--- end
--- :=
--- begin
---   ext1,
---   simp [has_add.add, add, has_lift.lift, lift],
--- end
-
-end cost_function
-
--- witness checks if the program provided is accepted by the cost function for all inputs
--- since cost_function is monotonic on the cost, this is a less than or equal relationship
-def witness: Π (enf : encodable_function m), α → enf.unwrap → (cost_function enf) → Prop
-| (encodable_function.result en) := λ prog data, en.model.accepts_with_cost prog (en.encode data)
-| (encodable_function.application en b) := λ prog f cost, ∀ arg : en.type,
-  witness b (encoding.application en prog arg) (f arg) (cost arg)
-
-
-theorem witness_trans (enf: encodable_function m) {cf cg: cost_function enf}:
-  ∀ {prog: α} {f: enf.unwrap}, cf ≤ cg → witness enf prog f cf → witness enf prog f cg :=
-begin
-  induction enf generalizing cf cg;
-  intros prog f hc,
-  { exact model.cost_mono m hc },
-  intros hf arg,
-  exact enf_ih (hc _) (hf _),
-end
-  
-def witness' (m: model α β γ) {δ: Type} [enf: has_encodable_function m δ] (prog: α) (f: δ) (cf: cost_function enf.value.value) :=
-  witness enf.value.value prog (cast_unwrap f) cf
-
-def complexity_le [enf: has_encodable_function m δ] (f: δ) (cf: cost_function enf.value.value) :=
-  ∃ prog: α, witness enf.value.value prog (cast_unwrap f) cf
-
-theorem complexity_le_trans (m: model α β γ) [enf: has_encodable_function m δ] {f: δ} {cf cg: cost_function enf.value.value}:
-  cf ≤ cg → complexity_le f cf → complexity_le f cg :=
-begin
-  intros mono hcf,
-  cases hcf with prog witness,
-  exact ⟨prog, witness_trans _ mono witness⟩
-end
-
-structure is_complexity (m: model α β γ) {δ: Type} [has_encodable_function m δ] (f: δ) :=
-mk ::
-  (cost : cost_function' m δ)
-  (proof : complexity_le f cost)
-
-class has_complexity (m: model α β γ) {δ: Type} [has_encodable_function m δ] (f: δ) :=
-  (value: is_complexity m f)
-
-theorem omega_equiv  {m: model α β γ} {δ: Type} [enf: has_encodable_function m δ] {f: δ} {cf: cost_function enf.value.value}:
-  complexity_le f cf → ∀ g, f = g → complexity_le g cf :=
-begin
-  intros hf g hfg,
-  rw [← hfg],
-  exact hf,
-end
+inductive witness
+  (m: complexity.model): Π {α β: Type*}, m.Program → α → β → Prop
+| result {α: Type*} [complexity.has_encoding α m.Result] (p: m.Program) (c: m.Cost) (ret: α)
+  (hc: m.has_cost p c) (hr: (m.result hc) = complexity.encode ret): witness p ret c
+| apply {α: Type*} {β: Type*} {γ: Type*} [complexity.has_encoding α m.Data] (p: m.Program) (f: α → β) (fc: α → γ)
+  (harg: Π (a: α), witness (m.apply p (complexity.encode a)) (f a) (fc a)): witness p f fc
 
 end complexity
 
-def complexity {α β γ: Type} [has_equiv β] [preorder γ] [has_add γ]
-  (m: complexity.model α β γ) {δ: Type} [complexity.has_encodable_function m δ]
-  (f: δ) [c: complexity.has_complexity m f]:
-  complexity.cost_function' m δ := c.value.cost
-
-instance {α β γ: Type} [has_equiv β] [preorder γ] [has_add γ] (m: complexity.model α β γ)
-  (δ: Type) [complexity.has_encodable_function m δ]:
-  has_le (complexity.cost_function' m δ) :=
-  ⟨ complexity.cost_function.less_than_or_equal ⟩
-
-def complexity_of_instance {α β γ: Type} [has_equiv β] [preorder γ] [has_add γ]
-  (m: complexity.model α β γ) {δ: Type} [enf: complexity.has_encodable_function m δ]
-  (f: δ) [c: complexity.has_complexity m f] (cf: complexity.cost_function' m δ):
-  c.value.cost ≤ cf → complexity.complexity_le f cf :=
- λ mono, complexity.complexity_le_trans m mono c.value.proof
-
+structure complexity {α β: Type*} (m: complexity.model) (f: α) (cost: β) :=
+  (program: m.Program)
+  (pf: complexity.witness m program f cost)
