src/hmem/encoding/basic.lean
@@ -17,62 +17,74 @@ def build_arg: list (memory μ) → memory μ
 | [m] := m
 | (x::xs) := push_arg (build_arg xs) x
 
-def runtime_model (μ: Type*) [decidable_eq μ] [has_zero μ] [has_one μ] [ne_zero (1:μ)]: complexity.model (program μ × list (memory μ)) (memory μ) ℕ :=
- ⟨  λ p_a r c, p_a.fst.has_result (build_arg p_a.snd) r ∧ p_a.fst.has_time_cost (build_arg p_a.snd) c,
-    λ p_a a', (p_a.fst, a'::p_a.snd),
-    λ _ _ _ _ _ hrc₁ hrc₂, program.unique_result hrc₁.left hrc₂.left,
-    λ _ _ _ _ hc hrc₀, ⟨hrc₀.left, program.time_cost_mono hrc₀.right hc⟩ ⟩
+def runtime_model (μ: Type*) [decidable_eq μ] [has_zero μ] [has_one μ] [ne_zero (1:μ)]: complexity.model :=
+⟨ (program μ × list (memory μ)),
+  memory μ,
+  memory μ,
+  ℕ,
+  ⟨ (=), eq.refl, @eq.symm _, @eq.trans _ ⟩,
+  ⟨ (=), eq.refl, @eq.symm _, @eq.trans _ ⟩,
+  infer_instance,
+  infer_instance,
+  λ p_a a, (p_a.fst, a::p_a.snd),
+  λ p_a, p_a.fst.has_time_cost (build_arg p_a.snd),
+  λ p_a _ h, program.result p_a.fst (build_arg p_a.snd) ⟨_, h⟩,
+  λ _ _, le_self_add,
+  λ _ _ _ hrc₀ hc, program.time_cost_mono hrc₀ hc ⟩
 
-def encode {δ: Type} [complexity.has_encoding (runtime_model μ) δ]: δ → memory μ := complexity.encode (runtime_model μ)
+theorem memory_equiv_eq_iff (μ: Type*) [decidable_eq μ] [has_zero μ] [has_one μ] [ne_zero (1:μ)] (m m': (runtime_model μ).Data):
+  ⟦m⟧ = ⟦m'⟧ ↔ m = m' := ⟨quotient.exact, λ h, h ▸ rfl⟩
 
-theorem encode_inj {δ: Type} [en: complexity.has_encoding (runtime_model μ) δ] {a b: δ}:
-  @encode μ _ _ _ _ δ _ a = encode b → a = b :=
-(en.value.encode_inj _ _).mp
+@[reducible]
+def encode {α: Type*} [complexity.has_encoding α (runtime_model μ).Data]: α → memory μ := @complexity.encode _ _ (runtime_model μ).data_equiv _
 
-instance (α β: Type*)  [α_en: complexity.has_encoding (runtime_model μ) α] [β_en: complexity.has_encoding (runtime_model μ) β]:
-  complexity.has_encoding (runtime_model μ) (α × β) :=
+@[reducible]
+def has_encoding (α: Type*) (μ: Type*) [decidable_eq μ] [has_zero μ] [has_one μ] [ne_zero (1:μ)] := complexity.has_encoding α (runtime_model μ).Data
+
+theorem encode_inj {α: Type*} [has_encoding α μ] {a b: α}: (encode a:memory μ) = encode b → a = b :=
 begin
-  fconstructor,
+  rw [← memory_equiv_eq_iff],
+  exact complexity.encode_inj,
+end
+
+theorem encode_inj' {α: Type*} (μ: Type*) [decidable_eq μ] [has_zero μ] [has_one μ] [ne_zero (1:μ)]  [has_encoding α μ] {a b: α}: (encode a:memory μ) = encode b → a = b :=
+begin
+  rw [← memory_equiv_eq_iff],
+  exact complexity.encode_inj,
+end
+
+instance prod_encoding (α β: Type*) [α_en: has_encoding α μ] [β_en: has_encoding β μ]:
+  has_encoding (α × β) μ :=
+begin
   fconstructor,
   exact λ ab, push_arg (encode ab.fst) (encode ab.snd),
   intros x y,
   cases x,
   cases y,
-  simp [push_arg, has_equiv.equiv, encode],
+  rw [memory_equiv_eq_iff, prod.eq_iff_fst_eq_snd_eq],
+  unfold push_arg,
+  intro h;
   split,
-  { intro h,
-    split,
-    { rw ← complexity.encoding.encode_inj α_en.value,
-      apply memory.getm_congr 0 h,
-      { rw [memory.getm_setm_ne _ _ _ _ zero_ne_one, memory.getm_setm],
-        refl,
-        apply_instance},
-      { rw [memory.getm_setm_ne _ _ _ _ zero_ne_one, memory.getm_setm],
-        refl,
-        apply_instance} },
-    { rw ← complexity.encoding.encode_inj β_en.value,
-      apply memory.getm_congr 1 h,
-      { rw [memory.getm_setm],
-        refl },
-      { rw [memory.getm_setm],
-        refl } } },
-  { intro h,
-    rw [h.left, h.right] }
+  { apply encode_inj' μ,
+    apply memory.getm_congr 0 h;
+    rw [memory.getm_setm_nz, memory.getm_setm] },
+  { apply encode_inj' μ,
+    apply memory.getm_congr 1 h;
+    rw [memory.getm_setm] }
 end
 
-theorem encode_pair  {α β: Type*}  [α_en: complexity.has_encoding (runtime_model μ) α] [β_en: complexity.has_encoding (runtime_model μ) β] (a: α) (b: β):
+theorem encode_pair  {α β: Type*}  [α_en: has_encoding α μ] [β_en: has_encoding β μ] (a: α) (b: β):
   encode (a, b) = (((memory.null μ).setv 1).setm 0 (encode a)).setm 1 (encode b) := rfl
 
-instance (p: Prop):
-  complexity.has_encoding (runtime_model μ) (decidable p) :=
+instance decidable_encoding (p: Prop):
+  has_encoding (decidable p) μ :=
 begin
-  fconstructor,
   fconstructor,
   exact λ d,  (memory.null _).setv (d.cases_on (λ _, 0) (λ _, 1)),
   intros x y,
   cases x;
   cases y;
-  simp [has_equiv.equiv, memory.setv_inj_iff],
+  simp [memory_equiv_eq_iff, memory.setv_inj_iff],
 end
 
 theorem encode_is_false {p: Prop} {hp: ¬ p} (d: decidable p):
@@ -81,71 +93,70 @@ theorem encode_is_false {p: Prop} {hp: ¬ p} (d: decidable p):
 theorem encode_is_true {p: Prop} {hp: p} (d: decidable p):
   (encode (is_true hp)) = (memory.null μ).setv 1 := rfl
 
-instance: complexity.has_encoding (runtime_model μ) bool :=
+instance bool_encoding: has_encoding bool μ :=
 begin
-  fconstructor,
   fconstructor,
   exact λ b,  (memory.null _).setv (ite b 1 0),
   intros x y,
   cases x;
   cases y;
-  simp [has_equiv.equiv, memory.setv_inj_iff],
+  simp [memory_equiv_eq_iff, memory.setv_inj_iff],
 end
 
-structure encodable_function (μ: Type*) [decidable_eq μ] [has_zero μ] [has_one μ] [ne_zero (1:μ)] :=
-  {α: Type} (α_en: complexity.encoding (runtime_model μ) α)
-  {β: Type} (β_en: complexity.encoding (runtime_model μ) β)
-  (f: α → β)
+-- structure encodable_function (μ: Type*) [decidable_eq μ] [has_zero μ] [has_one μ] [ne_zero (1:μ)] :=
+--   {α: Type} (α_en: complexity.encoding (runtime_model μ) α)
+--   {β: Type} (β_en: complexity.encoding (runtime_model μ) β)
+--   (f: α → β)
 
-structure encodable_application (μ: Type*) [decidable_eq μ] [has_zero μ] [has_one μ] [ne_zero (1:μ)] :=
-  {α: Type} (α_en: complexity.encoding (runtime_model μ) α)
-  {β: Type} (β_en: complexity.encoding (runtime_model μ) β)
-  (f: α → β)
-  (a: α)
+-- structure encodable_application (μ: Type*) [decidable_eq μ] [has_zero μ] [has_one μ] [ne_zero (1:μ)] :=
+--   {α: Type} (α_en: complexity.encoding (runtime_model μ) α)
+--   {β: Type} (β_en: complexity.encoding (runtime_model μ) β)
+--   (f: α → β)
+--   (a: α)
 
-structure encoded_function (μ: Type*) [decidable_eq μ] [has_zero μ] [has_one μ] [ne_zero (1:μ)] :=
-  {α: Type} (α_en: complexity.encoding (runtime_model μ) α)
-  {β: Type} (β_en: complexity.encoding (runtime_model μ) β)
-  (f: α → β)
-  (p: program μ)
-  (pf: ∀ a : α, p.has_result (α_en.encode a) (β_en.encode (f a)))
+-- structure encoded_function (μ: Type*) [decidable_eq μ] [has_zero μ] [has_one μ] [ne_zero (1:μ)] :=
+--   {α: Type} (α_en: complexity.encoding (runtime_model μ) α)
+--   {β: Type} (β_en: complexity.encoding (runtime_model μ) β)
+--   (f: α → β)
+--   (p: program μ)
+--   (pf: ∀ a : α, p.has_result (α_en.encode a) (β_en.encode (f a)))
 
-def program.call_structure_helper: program μ → ℕ → tree ℕ
-| [] n := tree.node n tree.nil tree.nil 
-| (@instruction.ite _ _ _ _ _ is'::is) n := tree.node n (program.call_structure_helper is 0) (program.call_structure_helper is' 0)
-| (instruction.call _ _ _::is) n := program.call_structure_helper is (n+1)
-| (i::is) n := program.call_structure_helper is n
+-- def program.call_structure_helper: program μ → ℕ → tree ℕ
+-- | [] n := tree.node n tree.nil tree.nil 
+-- | (@instruction.ite _ _ _ _ _ is'::is) n := tree.node n (program.call_structure_helper is 0) (program.call_structure_helper is' 0)
+-- | (instruction.call _ _ _::is) n := program.call_structure_helper is (n+1)
+-- | (i::is) n := program.call_structure_helper is n
 
-def program.call_structure: program μ → tree ℕ := flip program.call_structure_helper 0
+-- def program.call_structure: program μ → tree ℕ := flip program.call_structure_helper 0
 
-def tree.all₂ {α β: Type*} (f: α → β → Prop): tree α → tree β → Prop
-| tree.nil tree.nil := true
-| (tree.node a la ra) (tree.node b lb rb) := f a b ∧ tree.all₂ la lb ∧ tree.all₂ ra rb
-| _ _ := false
+-- def tree.all₂ {α β: Type*} (f: α → β → Prop): tree α → tree β → Prop
+-- | tree.nil tree.nil := true
+-- | (tree.node a la ra) (tree.node b lb rb) := f a b ∧ tree.all₂ la lb ∧ tree.all₂ ra rb
+-- | _ _ := false
 
-instance {α β: Type*} (f: α → β → Prop) [fd: Π {a b}, decidable (f a b)] (as: tree α) (bs: tree β):
-  decidable (tree.all₂ f as bs) :=
-begin
-  induction as with _ _ _ lhs_ih rhs_ih generalizing bs,
-  { cases bs,
-    exact decidable.is_true trivial,
-    exact decidable.is_false not_false },
-  { cases bs,
-    exact decidable.is_false not_false,
-    cases fd,
-    exact decidable.is_false (not_and_of_not_left _ h),
-    cases lhs_ih _,
-    exact decidable.is_false (not_and_of_not_right _ (not_and_of_not_left _ h_1)),
-    cases rhs_ih _,
-    exact decidable.is_false (not_and_of_not_right _ (not_and_of_not_right _ h_2)),
-    exact decidable.is_true ⟨h, h_1, h_2⟩}
-end
+-- instance {α β: Type*} (f: α → β → Prop) [fd: Π {a b}, decidable (f a b)] (as: tree α) (bs: tree β):
+--   decidable (tree.all₂ f as bs) :=
+-- begin
+--   induction as with _ _ _ lhs_ih rhs_ih generalizing bs,
+--   { cases bs,
+--     exact decidable.is_true trivial,
+--     exact decidable.is_false not_false },
+--   { cases bs,
+--     exact decidable.is_false not_false,
+--     cases fd,
+--     exact decidable.is_false (not_and_of_not_left _ h),
+--     cases lhs_ih _,
+--     exact decidable.is_false (not_and_of_not_right _ (not_and_of_not_left _ h_1)),
+--     cases rhs_ih _,
+--     exact decidable.is_false (not_and_of_not_right _ (not_and_of_not_right _ h_2)),
+--     exact decidable.is_true ⟨h, h_1, h_2⟩}
+-- end
 
-def tree.path {α: Type*}: tree α → list bool → list α
-| (tree.nil) _ := []
-| (tree.node a lhs rhs) [] := [a]
-| (tree.node a lhs rhs) (ff::p) := a :: tree.path lhs p
-| (tree.node a lhs rhs) (tt::p) := a :: tree.path rhs p
+-- def tree.path {α: Type*}: tree α → list bool → list α
+-- | (tree.nil) _ := []
+-- | (tree.node a lhs rhs) [] := [a]
+-- | (tree.node a lhs rhs) (ff::p) := a :: tree.path lhs p
+-- | (tree.node a lhs rhs) (tt::p) := a :: tree.path rhs p
 
 -- def makes_calls (μ: Type*) [decidable_eq μ] [has_zero μ] [has_one μ] [ne_zero (1:μ)]
 --   {α: Type} [complexity.has_encoding (runtime_model μ) α]
